added def for bmap with increasig bounds

leapfrog_project/lf_harm_lemmas.v
@@ -18,6 +18,9 @@ Import ListNotations.
 Definition _x : AST.ident := 1121%positive.
 Definition _v : AST.ident := 1117%positive.
 
+Definition x_init := float32_of_Z 0.
+Definition v_init := float32_of_Z 1.
+
 Import FPLangOpt. 
 Import FPLang.
 Import FPSolve.
@@ -30,13 +33,176 @@ Definition v' := ltac:(let e' :=
   HO_reify_float_expr constr:([_x; _v]) leapfrog_stepv in exact e').
 
 
-Definition leapfrog_bmap_list := 
-  [(_v, {|Test.var_type:=Tsingle; Test.var_name:=_v; Test.var_lobound:=-1; Test.var_hibound:=1|});
-  (_x,{|Test.var_type:=Tsingle; Test.var_name:=_x; Test.var_lobound:=-1; Test.var_hibound:=1|})].
+Fixpoint mk_bounds_list (id_list: list  (AST.ident * (type * (R * R)))) : ( list  (AST.ident * Test.varinfo))  :=
+  match id_list with
+  | t :: t' => let i := fst t in let ty:= fst ( snd t) in let r1:= fst (snd ( snd t)) in let r2:= snd (snd ( snd t))  in 
+      [(i, Build_varinfo ty i r1 r2)] ++ mk_bounds_list t'
+  | nil => []
+end.
+
+Definition leapfrog_bmap_list := mk_bounds_list [(_x, (Tsingle, (-1,1))); (_v, (Tsingle, (-1,1)))].
 Definition leapfrog_vmap_list (x v : float32) := [(_x, Values.Vsingle x);(_v, Values.Vsingle v)].
 Definition leapfrog_env  := (fun x v => list_to_bound_env leapfrog_bmap_list (leapfrog_vmap_list x v)). 
 Definition leapfrog_bmap :=  Maps.PTree_Properties.of_list leapfrog_bmap_list.
 Definition leapfrog_vmap (x v : float32) := Maps.PTree_Properties.of_list (leapfrog_vmap_list x v).
+
+Definition lf_bmap_list_n (erx erv: R) (n: nat) := 
+  mk_bounds_list [(_x, (Tsingle, (- 1 * (1 + INR n * erx ), 1 *( 1+  INR n * erx) ))); 
+                  (_v, (Tsingle, (-1 * (1 + INR n * erv ), 1* (1 + INR n * erv ))))].
+Definition lf_bmap_n (erx erv: R) (n: nat) :=  
+  Maps.PTree_Properties.of_list (lf_bmap_list_n erx erv n).
+Definition lf_vmap := Maps.PTree_Properties.of_list (leapfrog_vmap_list x_init v_init).
+Definition lf_env_n  (x v : float32) (ex ev: R) (n: nat) := 
+  list_to_bound_env (lf_bmap_list_n ex ev n) (leapfrog_vmap_list x v). 
+
+Lemma bmd_Sn_varinfo : 
+forall e1 e2 : R, 
+forall n: nat,
+forall i,
+forall v1 : varinfo,
+Maps.PTree.get i (lf_bmap_n e1 e2 ( n)) = Some v1 -> 
+exists v2 : varinfo,
+Maps.PTree.get i (lf_bmap_n e1 e2 (S n)) = Some v2.  
+Proof.
+intros.
+apply Maps.PTree.elements_correct in H.
+destruct H.
++ inversion H. 
+exists ({|
+       var_type := Tsingle;
+       var_name := _x;
+       var_lobound := -1 * (1 + INR (S n) * e1);
+       var_hibound := 1 * (1 + INR (S n) * e1)
+     |}).
+simpl; auto.
++ simpl in H. destruct H; try contradiction.
+inversion H. 
+exists ({|
+       var_type := Tsingle;
+       var_name := _v;
+       var_lobound := -1 * (1 + INR (S n) * e2);
+       var_hibound := 1 * (1 + INR (S n) * e2)
+     |}).
+simpl; auto. 
+Qed.
+
+Lemma bmd_Sn_exists_iff : 
+forall e1 e2 : R, 
+forall n: nat,
+forall i,
+(exists v1 : varinfo,
+Maps.PTree.get i (lf_bmap_n e1 e2 ( n)) = Some v1) <-> 
+(exists v2 : varinfo,
+Maps.PTree.get i (lf_bmap_n e1 e2 (S n)) = Some v2).  
+Proof.
+intros.
+split.
+intros. destruct H. eapply bmd_Sn_varinfo. apply H.
+intros. destruct H.
+apply Maps.PTree.elements_correct in H.
+destruct H.
++ inversion H. 
+exists ({|
+       var_type := Tsingle;
+       var_name := _x;
+       var_lobound := -1 * (1 + INR (n) * e1);
+       var_hibound := 1 * (1 + INR (n) * e1)
+     |}).
+simpl; auto.
++ simpl in H. destruct H; try contradiction.
+inversion H. 
+exists ({|
+       var_type := Tsingle;
+       var_name := _v;
+       var_lobound := -1 * (1 + INR ( n) * e2);
+       var_hibound := 1 * (1 + INR (n) * e2)
+     |}).
+simpl; auto. 
+Qed.
+
+
+Lemma bmd_Sn_vars_eq : 
+forall e1 e2 : R, 
+forall n: nat,
+forall i,
+forall v1 v2 : varinfo,
+Maps.PTree.get i (lf_bmap_n e1 e2 (S n)) = Some v1 -> 
+Maps.PTree.get i (lf_bmap_n e1 e2 ( n)) = Some v2 -> 
+v1.(var_name) = v2.(var_name) /\
+v1.(var_type) = v2.(var_type).
+Proof.
+intros.
+apply Maps.PTree.elements_correct in H.
+destruct H.
++ inversion H. subst. clear H.
+simpl in H0. inversion H0; auto.
++ simpl in H. destruct H; try contradiction.
+inversion H. subst. clear H.
+simpl in H0. inversion H0; auto. 
+Qed.
+
+
+
+Lemma bmd_Sn_bnds_le : 
+forall e1 e2 : R, 
+   0<= e1 ->
+   0<= e2 ->
+forall n: nat,
+forall i,
+forall v1 v2 : varinfo,
+Maps.PTree.get i (lf_bmap_n e1 e2 (S n)) = Some v1-> 
+Maps.PTree.get i (lf_bmap_n e1 e2 ( n)) = Some v2 -> 
+v1.(var_lobound) <= v2.(var_lobound) /\ 
+v2.(var_hibound) <= v1.(var_hibound). 
+Proof.
+intros.
+apply Maps.PTree.elements_correct in H1.
+inversion H1.
++ set (yy:= INR (S n)) in H3. inversion H3. subst. clear H1. 
+simpl in H2. inversion H2. simpl. subst yy. rewrite ?S_INR.
+split. all : (field_simplify; try nra).
++ set (yy:= INR (S n)) in H3. simpl in H3. destruct H3; try contradiction.
+inversion H3. subst. clear H1. 
+simpl in H2. inversion H2. simpl. subst yy. rewrite ?S_INR. 
+split. all : (field_simplify; try nra).
+Qed.
+
+
+Lemma bmd_Sn : 
+forall x v : float32, 
+forall e1 e2 : R, 
+0<= e1  ->
+0<= e2  ->
+forall n: nat,
+boundsmap_denote (lf_bmap_n e1 e2 (n)) (leapfrog_vmap x v) ->
+boundsmap_denote (lf_bmap_n e1 e2 (S n)) (leapfrog_vmap x v).
+Proof.
+intros.
+unfold boundsmap_denote.
+intros.
+ specialize (H1 i).
+pose proof bmd_Sn_bnds_le e1 e2 H H0 n i.
+pose proof bmd_Sn_vars_eq e1 e2 n i.
+pose proof bmd_Sn_exists_iff  e1 e2 n i.
+destruct (Maps.PTree.get i (leapfrog_vmap x v)).
++ destruct (Maps.PTree.get i (lf_bmap_n e1 e2 ( n))); try contradiction.
+++ destruct (Maps.PTree.get i (lf_bmap_n e1 e2 (S n))).
++++ specialize (H2 v2 v1 eq_refl eq_refl).
+specialize (H3 v2 v1  eq_refl eq_refl).
+destruct v1; destruct v2. 
+destruct H1 as (xp & A & B & C & D).
+simpl in H2; simpl in H3. destruct H3. subst.
+exists xp; repeat split; auto.
+eapply Rle_trans. apply H2. apply D.
+eapply Rle_trans. apply D. apply H2.
++++ destruct H4; destruct H4. exists v1; auto. discriminate; auto.
++ destruct (Maps.PTree.get i (lf_bmap_n e1 e2 ( n))).
+++  destruct v0; try contradiction.
+++ destruct (Maps.PTree.get i (lf_bmap_n e1 e2 (S n))); auto.
+destruct H4; destruct H5. exists v0; auto. discriminate; auto.
+Qed.
+
+
 
 Import B_Float_Notations.
 
@@ -44,6 +210,18 @@ Import B_Float_Notations.
 Lemma env_fval_reify_correct_leapfrog_step_x:
   forall x v : float32,
   fval (leapfrog_env x v) x' = leapfrog_stepx x v.
+Proof.
+intros. 
+unfold_reflect' x'.  
+unfold_float_ops_for_equality. 
+reflexivity.
+Qed.  
+
+Lemma env_n_fval_reify_correct_leapfrog_step_x:
+  forall x v : float32,
+  forall e1 e2 : R,
+  forall n : nat,
+  fval (lf_env_n x v e1 e2 n) x' = leapfrog_stepx x v.
 Proof.
 intros. 
 unfold_reflect' x'.  
@@ -62,10 +240,39 @@ unfold_float_ops_for_equality.
 reflexivity. 
 Qed.  
 
+Lemma env_n_fval_reify_correct_leapfrog_step_v:
+  forall x v : float32,
+  forall x v : float32,
+  forall e1 e2 : R,
+  forall n : nat,
+  fval (lf_env_n x v e1 e2 n) v' = leapfrog_stepv x v.
+Proof.
+intros.
+unfold_reflect' v'.  
+unfold_float_ops_for_equality. 
+reflexivity. 
+Qed.  
+
+
 Lemma env_fval_reify_correct_leapfrog_step:
   forall x v : float32,
   fval (leapfrog_env x v) x' = leapfrog_stepx x v /\
   fval (leapfrog_env  x v) v' = leapfrog_stepv x v.
+Proof.
+intros. 
+unfold leapfrog_env.
+unfold leapfrog_env; split.
+- unfold_reflect' x'. unfold_float_ops_for_equality. reflexivity.
+- unfold_reflect' v'. unfold_float_ops_for_equality. reflexivity.
+Qed.
+
+
+Lemma env_n_fval_reify_correct_leapfrog_step:
+  forall x v : float32,
+  forall e1 e2 : R,
+  forall n : nat,
+  fval (lf_env_n x v e1 e2 n) x' = leapfrog_stepx x v /\
+  fval (lf_env_n x v e1 e2 n) v' = leapfrog_stepv x v.
 Proof.
 intros. 
 unfold leapfrog_env.
@@ -80,7 +287,7 @@ Lemma env_rval_reify_correct_leapfrog_stepx:
   forall x1 v1 : R,
   x1 = B2R _ _ x ->
   v1 = B2R _ _ v -> 
-  rval (leapfrog_env x v) (optimize_div x') = fst (leapfrog_stepR (x1,v1)).
+  rval (leapfrog_env x v) (optimize_div x') = fst (leapfrog_stepR' (x1,v1)).
 Proof.
 intros.
 unfold leapfrog_env.
@@ -88,17 +295,38 @@ simplify_shift_div_opt (optimize_div x').
 match goal with |- context [rval ?env ?e] =>
   unfold_reflect_rval e; cbv [id]
 end.
-unfold leapfrog_stepR, F, h, fst, snd; subst.
+unfold leapfrog_stepR', F, h, fst, snd; subst.
 cbv [fprec femax]; simpl.
 unfold Defs.F2R; simpl; nra.
 Qed.
+
+Lemma env_n_rval_reify_correct_leapfrog_stepx:
+  forall x v : float32,
+  forall x1 v1 : R,
+  forall e1 e2 : R,
+  x1 = B2R _ _ x ->
+  v1 = B2R _ _ v -> 
+  forall n : nat,
+  rval (lf_env_n x v e1 e2 n) (optimize_div x') = fst (leapfrog_stepR' (x1,v1)).
+Proof.
+intros.
+unfold leapfrog_env.
+simplify_shift_div_opt (optimize_div x'). unfold lf_env_n.
+match goal with |- context [rval ?env ?e] =>
+  unfold_reflect_rval e; cbv [id]
+end.
+unfold leapfrog_stepR', F, h, fst, snd; subst.
+cbv [fprec femax]; simpl.
+unfold Defs.F2R; simpl; nra.
+Qed.
+
 
 Lemma env_rval_reify_correct_leapfrog_stepv:
   forall x v : float32,
   forall x1 v1 : R,
   x1 = B2R _ _ x ->
   v1 = B2R _ _ v -> 
-  rval (leapfrog_env x v) (optimize_div v') = snd (leapfrog_stepR (x1,v1)).
+  rval (leapfrog_env x v) (optimize_div v') = snd (leapfrog_stepR' (x1,v1)).
 Proof.
 intros.
 unfold leapfrog_env.
@@ -107,7 +335,27 @@ match goal with |- context [rval ?env ?e] =>
   unfold_reflect_rval e; cbv [id]
 end.
 simpl; rewrite ?Z.pow_pos_fold. 
-unfold leapfrog_stepR, F, h, fst; subst.  
+unfold leapfrog_stepR', F, h, fst; subst.  
+cbv [fprec femax]; simpl.
+unfold Defs.F2R; simpl; nra.
+Qed.
+
+Lemma env_n_rval_reify_correct_leapfrog_stepv:
+  forall x v : float32,
+  forall x1 v1 : R,
+  forall e1 e2 : R,
+  x1 = B2R _ _ x ->
+  v1 = B2R _ _ v -> 
+  forall n : nat,
+  rval (lf_env_n x v e1 e2 n) (optimize_div v') = snd (leapfrog_stepR' (x1,v1)).
+Proof.
+intros.
+unfold leapfrog_env.
+simplify_shift_div_opt (optimize_div v'). unfold lf_env_n.
+match goal with |- context [rval ?env ?e] =>
+  unfold_reflect_rval e; cbv [id]
+end.
+unfold leapfrog_stepR', F, h, fst, snd; subst.
 cbv [fprec femax]; simpl.
 unfold Defs.F2R; simpl; nra.
 Qed.
@@ -115,7 +363,7 @@ Qed.
 
 Require Import Coq.Logic.FunctionalExtensionality.
 
-Lemma lf_env_eq: 
+Lemma leapfrog_env_eq: 
   forall x v : float32,
 boundsmap_denote leapfrog_bmap  (leapfrog_vmap x v) ->
 leapfrog_env x v = env_ (leapfrog_vmap x v).
@@ -131,6 +379,27 @@ apply functional_extensionality; intro i.
     (Maps.PTree.get i (Maps.PTree_Properties.of_list (leapfrog_vmap_list x v))) 
     as [v'|]; try contradiction; auto.
 Qed.
+
+
+Lemma lf_env_n_eq: 
+forall x v : float32, 
+  forall n : nat,
+  forall e1 e2 : R, 
+boundsmap_denote (lf_bmap_n e1 e2 n)  (leapfrog_vmap x v) ->
+lf_env_n x v e1 e2 n  = env_ (leapfrog_vmap x v). 
+Proof.
+intros. pose proof (env_mk_env (lf_bmap_n e1 e2 n)  (leapfrog_vmap x v) H). 
+replace (env_ (leapfrog_vmap x v)) with 
+  (mk_env (lf_bmap_n e1 e2 n)  (leapfrog_vmap x v)). 
+unfold lf_env_n, list_to_bound_env, mk_env, lf_bmap_n, leapfrog_vmap.
+apply functional_extensionality_dep; intro ty.
+apply functional_extensionality; intro i.
+ destruct (Maps.PTree.get i (Maps.PTree_Properties.of_list 
+    (lf_bmap_list_n e1 e2 n))) as [[t i' lo hi]|],
+    (Maps.PTree.get i (Maps.PTree_Properties.of_list (leapfrog_vmap_list x v))) 
+    as [v'|]; try contradiction; auto.
+Qed.
+
 
 Import Interval.Tactic.
 
@@ -154,6 +423,79 @@ try solve_one_eval_cond2;
 try interval).
 Qed.
 
+
+Lemma conds2_hold_optx_n:
+forall x v : float32, 
+  forall n : nat,
+  (n <=1000)%nat ->
+  forall e1 e2 : R, 
+   0<= e1 <= 1 ->
+   0<= e2 <= 1 ->
+  boundsmap_denote (lf_bmap_n e1 e2 n) (leapfrog_vmap x v)->
+ forall r si2 s p,
+    rndval_with_cond 0 (mempty (Tsingle, Normal)) (optimize_div x') = ((r, (si2, s)), p)  ->
+list_forall (eval_cond2 (mk_env (lf_bmap_n e1 e2 n) (leapfrog_vmap x v)) s) p.
+Proof.
+intros.
+apply boundsmap_denote_e in H2.
+rewrite list_forall_Forall in H2.
+rewrite list_forall_Forall.
+rndval_inversion; subst.
+fold Tsingle ; fold Tdouble.
+prepare_assumptions_about_free_variables.
+clear H3.
+
+
+assert ( 1 * (1 + INR n * e1) <= 1001).
+eapply Rle_trans.
+eapply Rmult_le_compat_l; try nra.
+eapply Rplus_le_compat_l; try nra.
+eapply Rle_trans.
+eapply Rmult_le_compat_l. 
+apply pos_INR.
+apply H0. rewrite Rmult_1_r. 
+apply le_INR in H; apply H.
+try (simpl;nra).
+assert (-1001 <= FT2R Tsingle val_x).
+apply Ropp_le_contravar in H2; auto.
+rewrite Ropp_mult_distr_l in H2.
+eapply Rle_trans.
+apply H2. 
+eapply Rle_trans.
+apply Hrange_x. apply Rle_refl.
+assert (FT2R Tsingle val_x <= 1001).
+eapply Rle_trans.
+apply Hrange_x.
+apply H2.
+
+assert ( 1 * (1 + INR n * e2) <= 1001).
+eapply Rle_trans.
+eapply Rmult_le_compat_l; try nra.
+eapply Rplus_le_compat_l; try nra.
+eapply Rle_trans.
+eapply Rmult_le_compat_l.
+apply pos_INR.
+apply H1. rewrite Rmult_1_r. 
+apply le_INR in H; apply H.
+try (simpl;nra).
+assert (-1001 <= FT2R Tsingle val_v).
+apply Ropp_le_contravar in H5; auto.
+rewrite Ropp_mult_distr_l in H5.
+eapply Rle_trans.
+apply H5. 
+eapply Rle_trans.
+apply Hrange_v. apply Rle_refl.
+assert (FT2R Tsingle val_v <= 1001).
+eapply Rle_trans.
+apply Hrange_v.
+apply H5.
+
+repeat (apply List.Forall_cons; try apply List.Forall_nil;
+try solve_one_eval_cond2; 
+try interval).
+Qed.
+
+
 Lemma conds2_hold_optv:
   forall x v : float32,
 boundsmap_denote (leapfrog_bmap ) (leapfrog_vmap x v)->
@@ -168,6 +510,78 @@ rewrite list_forall_Forall.
 rndval_inversion; subst.
 fold Tsingle ; fold Tdouble.
 prepare_assumptions_about_free_variables;
+repeat (apply List.Forall_cons; try apply List.Forall_nil;
+try solve_one_eval_cond2; 
+try interval).
+Qed. 
+
+
+Lemma conds2_hold_optv_n:
+forall x v : float32, 
+  forall n : nat,
+  (n <=1000)%nat ->
+  forall e1 e2 : R, 
+   0<= e1 <= 1 ->
+   0<= e2 <= 1 ->
+boundsmap_denote (lf_bmap_n e1 e2 n) (leapfrog_vmap x v)->
+ forall r si2 s p,
+    rndval_with_cond 0 (mempty (Tsingle, Normal)) (optimize_div v') = ((r, (si2, s)), p)  ->
+list_forall (eval_cond2 (mk_env (lf_bmap_n e1 e2 n) (leapfrog_vmap x v)) s) p.
+Proof.
+intros.
+apply boundsmap_denote_e in H2.
+rewrite list_forall_Forall in H2.
+rewrite list_forall_Forall.
+rndval_inversion; subst.
+fold Tsingle ; fold Tdouble.
+prepare_assumptions_about_free_variables.
+clear H3.
+
+assert ( 1 * (1 + INR n * e1) <= 1001).
+eapply Rle_trans.
+eapply Rmult_le_compat_l; try nra.
+eapply Rplus_le_compat_l; try nra.
+eapply Rle_trans.
+eapply Rmult_le_compat_l.
+apply pos_INR.
+apply H0. rewrite Rmult_1_r. 
+apply le_INR in H; apply H.
+try (simpl;nra).
+try nra.
+assert (-1001 <= FT2R Tsingle val_x).
+apply Ropp_le_contravar in H2; auto.
+rewrite Ropp_mult_distr_l in H2.
+eapply Rle_trans.
+apply H2. 
+eapply Rle_trans.
+apply Hrange_x. apply Rle_refl.
+assert (FT2R Tsingle val_x <= 1001).
+eapply Rle_trans.
+apply Hrange_x.
+apply H2.
+
+assert ( 1 * (1 + INR n * e2) <= 1001).
+eapply Rle_trans.
+eapply Rmult_le_compat_l; try nra.
+eapply Rplus_le_compat_l; try nra.
+eapply Rle_trans.
+eapply Rmult_le_compat_l; try nra.
+apply pos_INR.
+apply H1. rewrite Rmult_1_r.
+apply le_INR in H; apply H.
+try (simpl;nra).
+assert (-1001 <= FT2R Tsingle val_v).
+apply Ropp_le_contravar in H5; auto.
+rewrite Ropp_mult_distr_l in H5.
+eapply Rle_trans.
+apply H5. 
+eapply Rle_trans.
+apply Hrange_v. apply Rle_refl.
+assert (FT2R Tsingle val_v <= 1001).
+eapply Rle_trans.
+apply Hrange_v.
+apply H5.
+
 repeat (apply List.Forall_cons; try apply List.Forall_nil;
 try solve_one_eval_cond2; 
 try interval).
@@ -276,6 +690,7 @@ eapply rndval_with_cond_correct; auto; try apply H0.
 rewrite <- env_mk_env in lc2; auto.
 Qed.
 
+
 Lemma rndval_with_cond_correct_optv:
   forall x v : float32,
     boundsmap_denote (leapfrog_bmap ) (leapfrog_vmap x v)->
@@ -296,6 +711,67 @@ assert (listconds : forall i : cond, In i p -> eval_cond1 (env_ (leapfrog_vmap x
 eapply rndval_with_cond_correct; auto; try apply H0.
 rewrite <- env_mk_env in lc2; auto.
 Qed.
+
+
+Lemma rndval_with_cond_correct_optx_n:
+forall x v : float32, 
+  forall n : nat,
+  (n <=1000)%nat ->
+  forall e1 e2 : R, 
+   0<= e1 <= 1 ->
+   0<= e2 <= 1 ->
+boundsmap_denote (lf_bmap_n e1 e2 n) (leapfrog_vmap x v)->
+forall r si2 s p,
+    rndval_with_cond 0 (mempty (Tsingle, Normal)) (optimize_div x') = ((r, (si2, s)), p)  ->
+rndval_with_cond_result (env_ (leapfrog_vmap x v)) (optimize_div x') r si2 s
+.
+Proof.
+intros.
+assert
+(HFIN : 
+  forall ty i, is_finite (fprec ty) (femax ty) (env_ (leapfrog_vmap x v) ty i) = true) by
+apply (finite_env (lf_bmap_n e1 e2 n) (leapfrog_vmap x v) H2).
+assert 
+(lc2 : 
+  list_forall (eval_cond2 (mk_env (lf_bmap_n e1 e2 n) (leapfrog_vmap x v)) s) p).
+eapply conds2_hold_optx_n; auto; apply H3.
+assert (HVALID : expr_valid (optimize_div x') = true) by reflexivity.
+assert (listconds : forall i : cond, In i p -> eval_cond1 (env_ (leapfrog_vmap x v)) s i) by
+           leapfrog_conds1_hold (optimize_div x') lc2.
+eapply rndval_with_cond_correct; auto; try apply H3.
+rewrite <- env_mk_env in lc2; auto.
+Qed.
+
+
+Lemma rndval_with_cond_correct_optv_n:
+forall x v : float32, 
+  forall n : nat,
+  (n <=1000)%nat ->
+  forall e1 e2 : R, 
+   0<= e1 <= 1 ->
+   0<= e2 <= 1 ->
+boundsmap_denote (lf_bmap_n e1 e2 n) (leapfrog_vmap x v)->
+forall r si2 s p,
+    rndval_with_cond 0 (mempty (Tsingle, Normal)) (optimize_div v') = ((r, (si2, s)), p)  ->
+rndval_with_cond_result (env_ (leapfrog_vmap x v)) (optimize_div v') r si2 s
+.
+Proof.
+intros.
+assert
+(HFIN : 
+  forall ty i, is_finite (fprec ty) (femax ty) (env_ (leapfrog_vmap x v) ty i) = true) by
+apply (finite_env (lf_bmap_n e1 e2 n) (leapfrog_vmap x v) H2).
+assert 
+(lc2 : 
+  list_forall (eval_cond2 (mk_env (lf_bmap_n e1 e2 n) (leapfrog_vmap x v)) s) p).
+eapply conds2_hold_optv_n; auto; apply H3.
+assert (HVALID : expr_valid (optimize_div v') = true) by reflexivity.
+assert (listconds : forall i : cond, In i p -> eval_cond1 (env_ (leapfrog_vmap x v)) s i) by
+           leapfrog_conds1_hold (optimize_div x') lc2.
+eapply rndval_with_cond_correct; auto; try apply H3.
+rewrite <- env_mk_env in lc2; auto.
+Qed.
+
 
 Ltac lf_rewrites :=
 repeat match goal with |- context [(env_ ?vmap ?ty2 ?var)] =>
@@ -321,8 +797,28 @@ Ltac fvs_from_bndsmap_hyp H:=
   prepare_assumptions_about_free_variables
 .
 
+Ltac interval_solve :=
+match goal with |- context [Rabs (?v) <= _] =>
+  field_simplify v;
+repeat (try split; try interval)
+end;
+match goal with |- context [Rabs (?v) <= _] =>
+  interval_intro (Rabs v) upper
+end;
+try nra 
+.
 
-Ltac intro_absolute_error_bound ty kn bmd x v rndval_result:=
+Ltac simpl_pow :=
+replace 8388608 with (2 ^ Pos.to_nat 23) by (simpl; field_simplify; nra);
+assert  (2 <> 0) by lra;
+ repeat (rewrite <- powerRZ_pos_sub; auto); 
+repeat match goal with |-context[(Z.pos_sub ?a ?b)] =>
+set (yy:= (Z.pos_sub a b)); compute in yy;
+subst yy
+end
+.
+
+Ltac intro_absolute_error_bound_aux ty kn bmd x v rndval_result:=
 match goal with |- context [
     Rle (Rabs (?op (rval ?env ?e) 
    (B2R _ _ (fval ?env ?e)))) 
@@ -335,7 +831,7 @@ cbv [Datatypes.id] in Hty;
 repeat change (type_lub ty ty) with ty in Hty;
 unfold Hty in *; clear Hty;
 pose proof rndval_result (fval env e) as RESULT_A ;
-rewrite ?lf_env_eq in RESULT_A; auto;
+         (*rewrite ?leapfrog_env_eq in RESULT_A; auto;*)
  pose proof RESULT_A eq_refl as RESULT; clear RESULT_A ;
 clear rndval_result; 
 destruct RESULT as (HFIN & ERRORS); 
@@ -350,7 +846,7 @@ subst;
 fold ty in * ;
 get_eps_delts ;
 try (rewrite <- ERRORS; clear ERRORS);
-try (rewrite ?lf_env_eq; auto; rewrite <- ERRORS; clear ERRORS);
+try (rewrite ?leapfrog_env_eq; auto; rewrite <- ERRORS; clear ERRORS);
 match goal with
   | |- context [ reval _ _ (mget (mset ?M _ _)) ] =>
         let m := fresh "m" in
@@ -367,50 +863,14 @@ cbv[F2R Defs.F2R fone bpow radix_val radix2 Fexp Fnum];
 rewrite ?Zpower_pos_powerRZ; unfold powerRZ; rewrite ?powerRZ_pos_sub2;
 rewrite ?Rmult_1_l; rewrite ?Rmult_1_r; rewrite ?powerRZ_O; 
 try lra;
-lf_rewrites;
-match goal with |- context [Rabs (?v) <= _] =>
-  field_simplify v;
-repeat (try split; try interval)
-end;
-match goal with |- context [Rabs (?v) <= _] =>
-  interval_intro (Rabs v) upper
-end;
-try nra 
+lf_rewrites
 end.
 
+Ltac intro_absolute_error_bound ty kn bmd x v rndval_result:=
+intro_absolute_error_bound_aux ty kn bmd x v rndval_result;
+try interval_solve
+.
 
-(* lemma for energy error, for difference of squares on v *)
-Lemma one_step_sum_v:
-  forall x v : float32,
-    boundsmap_denote leapfrog_bmap (leapfrog_vmap x v)->
-    Rle (Rabs (Rplus (rval (leapfrog_env x v)  (optimize_div v')) 
-    (B2R _ _ (fval (leapfrog_env x v) (optimize_div v'))))) 
-         (4646570650113373 / 2251799813685248)%R.
-Proof.
-intros.
-(destruct (rndval_with_cond O (mempty  (Tsingle, Normal)) (optimize_div v')) 
-  as [[r [si2 s]] p] eqn:rndval).
-pose proof (rndval_with_cond_correct_optv x v H r si2 s p rndval)
-  as rndval_result. 
-intro_absolute_error_bound Tsingle Normal H x v rndval_result.
-Qed.
-
-
-(* lemma for energy error, for difference of squares on x *)
-Lemma one_step_sum_x:
-  forall x v : float32,
-    boundsmap_denote (leapfrog_bmap ) (leapfrog_vmap x v)->
-    Rle (Rabs (Rplus (rval (leapfrog_env  x v) (optimize_div x')) 
-   (B2R _ _ (fval (leapfrog_env  x v) (optimize_div x'))))) 
-         (4646536420130942 / 2251799813685248)%R.
-Proof.
-intros.
-(destruct (rndval_with_cond O (mempty  (Tsingle, Normal)) (optimize_div x')) 
-  as [[r [si2 s]] p] eqn:rndval).
-pose proof (rndval_with_cond_correct_optx x v H r si2 s p rndval)
-  as rndval_result.
-intro_absolute_error_bound Tsingle Normal H x v rndval_result.
-Qed.
 
 Lemma leapfrog_opt_stepx_is_finite:
   forall x v : float32,
@@ -435,7 +895,6 @@ clear rndval_result;
 destruct RESULT as (HFIN & ERRORS).
 apply HFIN.
 Qed.
-
 
 Lemma leapfrog_opt_stepv_is_finite:
   forall x v : float32,
@@ -480,5 +939,95 @@ Proof.
 intros; subst;
 apply is_finite_not_is_nan.
 apply leapfrog_opt_stepv_is_finite; auto. 
+Qed.
+
+
+Lemma leapfrog_opt_stepx_is_finite_n:
+forall x v : float32, 
+  forall n : nat,
+  (n <=1000)%nat ->
+  forall e1 e2 : R, 
+   0<= e1 <= 1 ->
+   0<= e2 <= 1 ->
+  boundsmap_denote (lf_bmap_n e1 e2 n) (leapfrog_vmap x v)->
+  Binary.is_finite _ _(fval (lf_env_n x v e1 e2 n) (optimize_div x')) = true.
+Proof.
+intros.
+(destruct (rndval_with_cond O (mempty  (Tsingle, Normal)) (optimize_div x')) 
+  as [[r [si2 s]] p] eqn:rndval).
+pose proof (rndval_with_cond_correct_optx_n x v n H e1 e2 H0 H1 H2 r si2 s p rndval)
+  as rndval_result. 
+unfold rndval_with_cond_result in rndval_result;
+set (Hty:= type_of_expr (optimize_div x')) in *.
+repeat simpl in Hty.
+cbv [Datatypes.id] in Hty.   
+repeat change (type_lub Tsingle Tsingle) with Tsingle in Hty;
+unfold Hty in *; clear Hty.
+pose proof rndval_result (fval (lf_env_n x v e1 e2 n) x') as RESULT_A ;
+rewrite ?lf_env_eq in RESULT_A; auto.
+ pose proof RESULT_A eq_refl as RESULT; clear RESULT_A ;
+clear rndval_result; 
+destruct RESULT as (HFIN & ERRORS).
+apply HFIN.
+Qed.
+
+Lemma leapfrog_opt_stepv_is_finite_n:
+forall x v : float32, 
+  forall n : nat,
+  (n <=1000)%nat ->
+  forall e1 e2 : R, 
+   0<= e1 <= 1 ->
+   0<= e2 <= 1 ->
+  boundsmap_denote (lf_bmap_n e1 e2 n) (leapfrog_vmap x v)->
+  Binary.is_finite _ _(fval (lf_env_n x v e1 e2 n) (optimize_div v')) = true.
+Proof.
+intros.
+(destruct (rndval_with_cond O (mempty  (Tsingle, Normal)) (optimize_div v')) 
+  as [[r [si2 s]] p] eqn:rndval).
+pose proof (rndval_with_cond_correct_optv_n x v n H e1 e2 H0 H1 H2 r si2 s p rndval)
+  as rndval_result. 
+unfold rndval_with_cond_result in rndval_result;
+set (Hty:= type_of_expr (optimize_div v')) in *.
+repeat simpl in Hty.
+cbv [Datatypes.id] in Hty.   
+repeat change (type_lub Tsingle Tsingle) with Tsingle in Hty;
+unfold Hty in *; clear Hty.
+pose proof rndval_result (fval (lf_env_n x v e1 e2 n) v') as RESULT_A ;
+rewrite ?lf_env_eq in RESULT_A; auto.
+ pose proof RESULT_A eq_refl as RESULT; clear RESULT_A ;
+clear rndval_result; 
+destruct RESULT as (HFIN & ERRORS).
+apply HFIN.
+Qed.
+
+
+Lemma leapfrog_stepx_not_nan_n:
+forall x v : float32, 
+  forall n : nat,
+  (n <= 1000)%nat ->
+  forall e1 e2 : R, 
+   0<= e1 <= 1 ->
+   0<= e2 <= 1 ->
+  boundsmap_denote (lf_bmap_n e1 e2 n) (leapfrog_vmap x v)->
+  Binary.is_nan _ _(fval (lf_env_n x v e1 e2 n) x') = false.
+Proof. 
+intros; subst;
+apply is_finite_not_is_nan.
+eapply leapfrog_opt_stepx_is_finite_n; auto.
+Qed.
+
+Lemma leapfrog_stepv_not_nan_n:
+forall x v : float32, 
+  forall n : nat,
+  (n <= 1000)%nat ->
+  forall e1 e2 : R, 
+   0<= e1 <= 1 ->
+   0<= e2 <= 1 ->
+  boundsmap_denote (lf_bmap_n e1 e2 n) (leapfrog_vmap x v)->
+  Binary.is_nan _ _(fval (lf_env_n x v e1 e2 n) v') = false.
+Proof. 
+intros; subst;
+apply is_finite_not_is_nan.
+eapply leapfrog_opt_stepv_is_finite_n; auto.
 Qed.
 
